src/ListMemoryZAddr.v
@@ -3,6 +3,7 @@
 Require Import Coq.Lists.List.
 Require Import bbv.Word.
 Require Import Coq.ZArith.ZArith.
+Require Import Coq.micromega.Lia.
 Require Import riscv.Utility.
 Require Import riscv.util.Monads.
 Require Import riscv.Memory.
@@ -10,80 +11,106 @@ Import ListNotations.
 Import Word.ArithmeticNotations.
 Import Word.ConversionNotations.
 Local Open Scope word_scope.
+Local Open Scope Z_scope.
+
 
 Section Memory.
 
   Definition mem := list (word 8).
-  Definition mem_size(m: mem): nat := length m.
+  Definition mem_size(m: mem): Z := Zlength m.
 
-  Definition read_byte(m: mem)(a: nat): word 8 := nth a m $0.
+  Definition read_byte(m: mem)(a: Z): word 8 := Znth m a $0.
 
-  Definition write_byte'(m: mem)(a: nat)(v: word 8): mem :=
-    (firstn a m) ++ [v] ++ (skipn (S a) m).
+  Definition write_byte'(m: mem)(a: Z)(v: word 8): mem :=
+    (Zfirstn a m) ++ [v] ++ (Zskipn (a + 1) m).
 
   (* fix for the case when a is out of bounds to make sure length is always preserved:
      allows for _preserves_mem_size lemmas with no hypotheses, and ensures things which
      should not work because out of bounds writes-then-reads don't work *)
-  Definition write_byte(m: mem)(a: nat)(v: word 8): mem :=
+  Definition write_byte(m: mem)(a: Z)(v: word 8): mem :=
     firstn (length m) (write_byte' m a v).
   
-  Definition read_half(m: mem)(a: nat): word 16 :=
+  Definition read_half(m: mem)(a: Z): word 16 :=
     let v0 := read_byte m a in let v1 := read_byte m (a + 1) in combine v0 v1.
-  Definition read_word(m: mem)(a: nat): word 32 :=
+  Definition read_word(m: mem)(a: Z): word 32 :=
     let v0 := read_half m a in let v1 := read_half m (a + 2) in combine v0 v1.
-  Definition read_double(m: mem)(a: nat): word 64 :=
+  Definition read_double(m: mem)(a: Z): word 64 :=
     let v0 := read_word m a in let v1 := read_word m (a + 4) in combine v0 v1.
 
   Definition lobits(sz: nat)(w: word (sz + sz)): word sz := split1 sz sz w.
   Definition hibits(sz: nat)(w: word (sz + sz)): word sz := split2 sz sz w.
 
-  Definition write_half(m: mem)(a: nat)(v: word 16): mem :=
+  Definition write_half(m: mem)(a: Z)(v: word 16): mem :=
     let m := write_byte m a (lobits 8 v) in write_byte m (a + 1) (hibits 8 v).
-  Definition write_word(m: mem)(a: nat)(v: word 32): mem :=
+  Definition write_word(m: mem)(a: Z)(v: word 32): mem :=
     let m := write_half m a (lobits 16 v) in write_half m (a + 2) (hibits 16 v).
-  Definition write_double(m: mem)(a: nat)(v: word 64): mem :=
+  Definition write_double(m: mem)(a: Z)(v: word 64): mem :=
     let m := write_word m a (lobits 32 v) in write_word m (a + 4) (hibits 32 v).
 
-  Fixpoint const_mem(default: word 8)(size: nat): mem :=
-    match size with
-    | O => []
-    | S n => default :: (const_mem default n)
-    end.
+  Definition const_mem(default: word 8)(size: Z): mem :=
+    map_range (fun _: Z => default) size.
 
   Lemma const_mem_mem_size: forall default size,
+      0 <= size ->
       mem_size (const_mem default size) = size.
   Proof.
-    intros. unfold mem_size. induction size; simpl; auto.
+    intros. unfold mem_size, const_mem. apply Zlength_map_range. assumption.
   Qed.
 
-  Definition zero_mem: nat -> mem := const_mem $0.
+  Definition zero_mem: Z -> mem := const_mem $0.
 
 End Memory.
 
+Ltac omega' := zify; rewrite Z2Nat.id in *; omega.
 
 Lemma write_read_byte_eq': forall m a1 a2 v,
-    a1 < mem_size m ->
+    0 <= a1 < mem_size m ->
     a2 = a1 ->
     read_byte (write_byte' m a1 v) a2 = v.
 Proof.
   intros. subst. unfold write_byte', read_byte, mem_size in *.
-  pose proof (@firstn_length_le _ m a1).
-  rewrite app_nth2 by omega.
-  rewrite H0 by omega.
-  replace (a1 - a1) with 0 by omega.
+  unfold Zfirstn, Zskipn, Znth, Zlength in *.
+  pose proof (@firstn_length_le _ m (Z.to_nat a1)).
+  rewrite app_nth2 by omega'.
+  rewrite H0 by omega'.
+  replace (Z.to_nat a1 - Z.to_nat a1)%nat with 0%nat by omega.
   reflexivity.
 Qed.
 
+Lemma Z_bounds_to_nat_bound: forall (a: Z) (n: nat),
+    0 <= a < Z.of_nat n ->
+    (Z.to_nat a < n)%nat.
+Proof.
+  intros. omega'.
+Qed.
+
+Lemma Z_ne_to_nat_ne: forall (a b: Z),
+    0 <= a ->
+    0 <= b ->
+    a <> b ->
+    Z.to_nat a <> Z.to_nat b.
+Proof.
+  intros. intro. apply H1. apply Z2Nat.inj; assumption.
+Qed.
+
 Lemma write_read_byte_ne': forall m a1 a2 v,
-    a1 < mem_size m ->
-    a2 < mem_size m ->
+    0 <= a1 < mem_size m ->
+    0 <= a2 < mem_size m ->
     a2 <> a1 ->
     read_byte (write_byte' m a1 v) a2 = read_byte m a2.
 Proof.
   intros. unfold write_byte', read_byte, mem_size in *.
-  pose proof (@firstn_length_le _ m a1).
-  pose proof (@firstn_length_le _ m a2).
-  assert (a2 < a1 \/ a1 < a2 < length m) as P by omega.
+  pose proof (@firstn_length_le _ m (Z.to_nat a1)).
+  pose proof (@firstn_length_le _ m (Z.to_nat a2)).
+  unfold Znth, Zfirstn, Zskipn, Zlength in *.
+  rewrite Z2Nat.inj_add by omega.
+  apply Z_ne_to_nat_ne in H1; [|omega..].
+  apply Z_bounds_to_nat_bound in H.
+  apply Z_bounds_to_nat_bound in H0.
+  remember (Z.to_nat a1) as a1'. clear Heqa1' a1. rename a1' into a1.
+  remember (Z.to_nat a2) as a2'. clear Heqa2' a2. rename a2' into a2.
+  replace (a1 + Z.to_nat 1)%nat with (S a1) by omega'.
+  assert (a2 < a1 \/ a1 < a2 < length m)%nat as P by omega.
   destruct P as [P | P].
   - rewrite app_nth1 by omega.
     clear H2 H3.
@@ -96,14 +123,14 @@ Proof.
   - rewrite app_nth2 by omega.
     rewrite app_nth2 by (simpl; omega).
     rewrite H2 by omega.
-    replace (a2 - a1 - length [v]) with (a2 - (S a1)) by (simpl; omega).
+    replace (a2 - a1 - length [v])%nat with (a2 - (S a1))%nat by (simpl; omega).
     clear H2 H3.
     generalize dependent m. generalize dependent a1.
     induction a2; intros.
     + omega.
-    + replace (S a2 - S a1) with (a2 - a1) by omega.
+    + replace (S a2 - S a1)%nat with (a2 - a1)%nat by omega.
       destruct a1.
-      * replace (a2 - 0) with a2 by omega. destruct m; [simpl in *; omega|reflexivity].
+      * replace (a2 - 0)%nat with a2 by omega. destruct m; [simpl in *; omega|reflexivity].
       * destruct m; [simpl in *; omega|].
         change (skipn (S (S a1)) (w :: m)) with (skipn (S a1) m).
         change (nth (S a2) (w :: m)) with (nth a2 m).
@@ -111,8 +138,8 @@ Proof.
 Qed.
 
 Lemma skipn_length_le: forall A n (l: list A),
-    n <= length l ->
-    length (skipn n l) = length l - n.
+    (n <= length l)%nat ->
+    length (skipn n l) = (length l - n)%nat.
 Proof.
   induction n; intros.
   - simpl. omega.
@@ -122,63 +149,97 @@ Proof.
 Qed.
 
 Lemma write_byte_preserves_mem_size': forall m a v,
-    a < mem_size m ->
+    0 <= a < mem_size m ->
     mem_size (write_byte' m a v) = mem_size m.
 Proof.
   intros. unfold mem_size, write_byte' in *.
+  unfold Zlength, Zfirstn, Zskipn in *.
   repeat rewrite app_length.
-  rewrite firstn_length_le by omega.
-  rewrite skipn_length_le by omega.
+  rewrite firstn_length_le by omega'.
+  rewrite skipn_length_le by omega'.
   simpl.
-  omega.
+  omega'.
+Qed.
+
+Lemma firstn_all_write_byte': forall m a1 v,
+    0 <= a1 < mem_size m ->
+    firstn (length m) (write_byte' m a1 v) = write_byte' m a1 v.
+Proof.
+  intros.
+  replace (length m) with (length (write_byte' m a1 v)).
+  - rewrite firstn_all. reflexivity.
+  - pose proof (write_byte_preserves_mem_size' m a1 v H) as P.
+    unfold mem_size, Zlength in *.
+    apply Nat2Z.inj in P.
+    assumption.
 Qed.
 
 Lemma write_read_byte_eq: forall m a1 a2 v,
-    a1 < mem_size m ->
+    0 <= a1 < mem_size m ->
     a2 = a1 ->
     read_byte (write_byte m a1 v) a2 = v.
 Proof.
   intros. unfold write_byte in *.
-  erewrite <- write_byte_preserves_mem_size' by eassumption.
-  unfold mem_size.
-  rewrite firstn_all.
-  apply write_read_byte_eq'; assumption.
+  erewrite <- write_read_byte_eq' by eassumption.
+  rewrite firstn_all_write_byte' by assumption.
+  reflexivity.
 Qed.
 
 Lemma write_read_byte_ne: forall m a1 a2 v,
-    a1 < mem_size m ->
-    a2 < mem_size m ->
+    0 <= a1 < mem_size m ->
+    0 <= a2 < mem_size m ->
     a2 <> a1 ->
     read_byte (write_byte m a1 v) a2 = read_byte m a2.
 Proof.
   intros. unfold write_byte in *.
-  erewrite <- write_byte_preserves_mem_size'; [|exact H].
-  unfold mem_size.
-  rewrite firstn_all.
-  apply write_read_byte_ne'; assumption.
+  rewrite <- (write_read_byte_ne' m a1 a2 v);
+    rewrite? firstn_all_write_byte' by assumption;
+    rewrite? write_byte_preserves_mem_size' by assumption;
+    [reflexivity | eassumption ..].
+Qed.
+
+Lemma Z2Nat_nonpos: forall (a: Z),
+    a <= 0 ->
+    Z.to_nat a = 0%nat.
+Proof.
+  intros.
+  destruct a.
+  - reflexivity.
+  - lia.
+  - apply Z2Nat.inj_neg.
 Qed.
 
 Lemma write_byte_preserves_mem_size: forall m a v,
     mem_size (write_byte m a v) = mem_size m.
 Proof.
   intros. unfold write_byte.
-  assert (a < mem_size m \/ a >= mem_size m) as C by omega. destruct C as [H | H].
+  assert (a < 0 \/ 0 <= a < mem_size m \/ a >= mem_size m) as C by omega.
+  destruct C as [H | [H | H]].
+  - unfold write_byte', Zfirstn, Zskipn.
+    rewrite! Z2Nat_nonpos by omega.
+    simpl.
+    unfold mem_size, Zlength in *.
+    apply Znat.inj_eq.
+    apply firstn_length_le.
+    simpl.
+    repeat constructor.
   - pose proof write_byte_preserves_mem_size' as P.
     specialize P with (1 := H).
-    unfold mem_size in *.
+    unfold mem_size, Zlength in *.
     rewrite <- (P v) at 1.
-    rewrite firstn_all.
-    apply P.
-  - unfold mem_size in *.
+    rewrite firstn_all_write_byte' by assumption.
+    reflexivity.
+  - unfold mem_size, Zlength in *.
+    apply Znat.inj_eq.
     apply firstn_length_le.
-    unfold write_byte'.
+    unfold write_byte', Zfirstn, Zskipn.
     rewrite? app_length.
     rewrite firstn_length.
-    pose proof (Nat.min_spec a (length m)).
-    omega.
+    omega'.
 Qed.
 
 Lemma write_read_half_eq: forall m a1 a2 v,
+    0 <= a1 ->
     a1 + 1 < mem_size m ->
     a2 = a1 ->
     read_half (write_half m a1 v) a2 = v.
@@ -200,6 +261,8 @@ Lemma write_read_half_ne: forall m a1 a2 v,
     a2 + 1 < mem_size m ->
     a2 mod 2 = 0 ->
     a2 <> a1 ->
+    0 <= a1 ->
+    0 <= a2 ->
     read_half (write_half m a1 v) a2 = read_half m a2.
 Proof.
   intros. unfold write_half, read_half in *.
@@ -208,13 +271,13 @@ Proof.
     + apply write_read_byte_ne; omega.
     + rewrite write_byte_preserves_mem_size; omega.
     + rewrite write_byte_preserves_mem_size; omega.
-    + intro. subst. rewrite Nat.add_mod in H2; try omega.
+    + intro. subst. rewrite Z.add_mod in H2; try omega.
       rewrite H0 in H2.
       simpl in H2.
       discriminate.
   - rewrite write_read_byte_ne.
     + apply write_read_byte_ne; try omega.
-      intro. subst. rewrite Nat.add_mod in H0; try omega.
+      intro. subst. rewrite Z.add_mod in H0; try omega.
       rewrite H2 in H0.
       simpl in H0.
       discriminate.
@@ -228,10 +291,10 @@ Lemma add_mod_r: forall a m,
     (a + m) mod m = a mod m.
 Proof.
   intros.
-  rewrite Nat.add_mod by assumption.
-  rewrite Nat.mod_same by assumption.
-  rewrite Nat.add_0_r.
-  apply Nat.mod_mod.
+  rewrite Z.add_mod by assumption.
+  rewrite Z.mod_same by assumption.
+  rewrite Z.add_0_r.
+  apply Z.mod_mod.
   assumption.
 Qed.
 
@@ -242,12 +305,10 @@ Lemma weaken_alignment: forall n al,
 Proof.
   intros.
   pose proof H.
-  apply Nat.mod_divides in H; try omega.
+  apply Z.mod_divide in H; try omega.
   destruct H as [n' H]. subst.
-  rewrite <- Nat.mul_assoc.
-  rewrite Nat.mul_mod by omega.
-  rewrite Nat.mod_same by assumption.
-  apply Nat.mod_0_l.
+  replace (n' * (al * 2)) with (n' * 2 * al) by ring.
+  apply Z.mod_mul.
   assumption.
 Qed.  
 
@@ -270,16 +331,17 @@ Lemma write_read_word_eq: forall m a1 a2 v,
     a1 + 4 <= mem_size m ->
     a1 mod 4 = 0 ->
     a2 = a1 ->
+    0 <= a1 ->
     read_word (write_word m a1 v) a2 = v.
 Proof.
   intros. subst. unfold write_word, read_word in *.
   pose proof H.
-  rewrite (write_read_half_eq _ (a1 + 2) (a1 + 2)); try reflexivity.
+  rewrite (write_read_half_eq _ (a1 + 2) (a1 + 2)); try reflexivity; try omega.
   - rewrite write_read_half_ne; try omega.
     + rewrite write_read_half_eq; try reflexivity; try omega.
       apply (combine_split 16 16).
     + rewrite write_half_preserves_mem_size; omega.
-    + apply diviBy4_implies_diviBy2 in H0. rewrite Nat.add_mod by omega.
+    + apply diviBy4_implies_diviBy2 in H0. rewrite Z.add_mod by omega.
       rewrite H0.
       reflexivity.
     + rewrite write_half_preserves_mem_size; omega.
@@ -293,28 +355,33 @@ Lemma write_read_word_ne: forall m a1 a2 v,
     a2 + 4 <= mem_size m ->
     a2 mod 4 = 0 ->
     a2 <> a1 ->
+    0 <= a1 ->
+    0 <= a2 ->
     read_word (write_word m a1 v) a2 = read_word m a2.
 Proof.
   intros. unfold write_word, read_word in *.
+  rename H4 into H6, H5 into H7.
   pose proof (diviBy4_implies_diviBy2 _ H0).
   pose proof (diviBy4_implies_diviBy2 _ H2).
   f_equal.
   - rewrite write_read_half_ne.
     + apply write_read_half_ne; omega.
     + rewrite write_half_preserves_mem_size; omega.
-    + rewrite Nat.add_mod by omega.
+    + rewrite Z.add_mod by omega.
       rewrite H4.
       reflexivity.
     + rewrite write_half_preserves_mem_size; omega.
     + assumption.
-    + intro. subst. rewrite Nat.add_mod in H2; try omega.
+    + intro. subst. rewrite Z.add_mod in H2; try omega.
       rewrite H0 in H2.
       simpl in H2.
       discriminate.
+    + omega.
+    + assumption.
   - rewrite write_read_half_ne.
     + apply write_read_half_ne; try omega.
       * rewrite add_mod_r; omega.
-      * intro. subst. rewrite Nat.add_mod in H0; try omega.
+      * intro. subst. rewrite Z.add_mod in H0; try omega.
         rewrite H2 in H0.
         simpl in H0.
         discriminate.
@@ -323,8 +390,9 @@ Proof.
     + rewrite write_half_preserves_mem_size; omega.
     + rewrite add_mod_r; omega.
     + omega.
+    + omega.
+    + omega.
 Qed.
-
 
 Lemma write_word_preserves_mem_size: forall m a v,
     mem_size (write_word m a v) = mem_size m.
@@ -345,17 +413,18 @@ Lemma write_read_double_eq: forall m a1 a2 v,
     a1 + 8 <= mem_size m ->
     a1 mod 8 = 0 ->
     a2 = a1 ->
+    0 <= a1 ->
     read_double (write_double m a1 v) a2 = v.
 Proof.
   intros. subst. unfold write_double, read_double in *.
   pose proof H.
-  rewrite (write_read_word_eq _ (a1 + 4) (a1 + 4)); try reflexivity.
+  rewrite (write_read_word_eq _ (a1 + 4) (a1 + 4)); try reflexivity; try omega.
   - rewrite write_read_word_ne; try omega.
     + rewrite write_read_word_eq; try reflexivity; try omega.
       * apply (combine_split 32 32).
       * apply diviBy8_implies_diviBy4. assumption.
     + rewrite write_word_preserves_mem_size; omega.
-    + apply diviBy8_implies_diviBy4 in H0. rewrite Nat.add_mod by omega.
+    + apply diviBy8_implies_diviBy4 in H0. rewrite Z.add_mod by omega.
       rewrite H0.
       reflexivity.
     + rewrite write_word_preserves_mem_size; omega.
@@ -371,28 +440,33 @@ Lemma write_read_double_ne: forall m a1 a2 v,
     a2 + 8 <= mem_size m ->
     a2 mod 8 = 0 ->
     a2 <> a1 ->
+    0 <= a1 ->
+    0 <= a2 ->
     read_double (write_double m a1 v) a2 = read_double m a2.
 Proof.
   intros. unfold write_double, read_double in *.
+  rename H4 into H6, H5 into H7.
   pose proof (diviBy8_implies_diviBy4 _ H0).
   pose proof (diviBy8_implies_diviBy4 _ H2).
   f_equal.
   - rewrite write_read_word_ne.
     + apply write_read_word_ne; omega.
     + rewrite write_word_preserves_mem_size; omega.
-    + rewrite Nat.add_mod by omega.
+    + rewrite Z.add_mod by omega.
       rewrite H4.
       reflexivity.
     + rewrite write_word_preserves_mem_size; omega.
     + assumption.
-    + intro. subst. rewrite Nat.add_mod in H2; try omega.
+    + intro. subst. rewrite Z.add_mod in H2; try omega.
       rewrite H0 in H2.
       simpl in H2.
       discriminate.
+    + omega.
+    + omega.
   - rewrite write_read_word_ne.
     + apply write_read_word_ne; try omega.
       * rewrite add_mod_r; omega.
-      * intro. subst. rewrite Nat.add_mod in H0; try omega.
+      * intro. subst. rewrite Z.add_mod in H0; try omega.
         rewrite H2 in H0.
         simpl in H0.
         discriminate.
@@ -400,6 +474,8 @@ Proof.
     + rewrite add_mod_r; omega.
     + rewrite write_word_preserves_mem_size; omega.
     + rewrite add_mod_r; omega.
+    + omega.
+    + omega.
     + omega.
 Qed.
 
